grouphomo.v
@@ -1,0 +1,33 @@
+From GRP Require Export group.
+From GRP Require Export groupop.
+
+Theorem homo_preserves_id :
+  forall (G1 G2 : group) (f : grp_homo G1 G2),
+    f (gr_id G1) = gr_id G2.
+Proof.
+  intros.
+  replace (gr_id G1) with (gr_op G1 (gr_id G1) (gr_inv G1 (gr_id G1))).
+  rewrite preserves_op. rewrite preserves_inv.
+  rewrite gr_inv_r. reflexivity.
+  rewrite gr_inv_r. reflexivity.
+  Qed.
+
+Definition kernel (G1 G2 : group) (f : grp_homo G1 G2) : subgroup_prop G1.
+Proof.
+  exists (fun g1 => f g1 = gr_id G2).
+  - apply homo_preserves_id.
+  - intros. rewrite preserves_op.
+    rewrite H. rewrite H0. rewrite gr_id_l. reflexivity.
+  - intros. rewrite preserves_inv. rewrite H.
+    apply grp_id_inv_id.
+  Qed.
+
+Definition image (G1 G2 : group) (f : grp_homo G1 G2) : subgroup_prop G2.
+Proof.
+  exists (fun g2 => exists g1, f g1 = g2).
+  - exists (gr_id G1). apply homo_preserves_id.
+  - intros. destruct H; destruct H0.
+    exists (gr_op G1 x x0). subst. apply preserves_op.
+  - intros. destruct H. exists (gr_inv G1 x).
+    subst. apply preserves_inv.
+  Qed.
